Finish proof of eq part
Separate stuff into definitions and lemmas
Prove all admitted except for the one we need to add
Refactor as axiom so no more admits
Comments in equality proof
Only 1 part left

proofs/transform/eliminate_inductive.v
@@ -652,6 +652,20 @@ Qed.
 
 (*TODO: can we prove this?*)
 
+
+(*Things about inductive predicates in general*)
+
+(*TODO: this one we need to add as assumption (either directly
+  or from assumption that can't have empty fs)*)
+(*TODO: use above*)
+Lemma indprop_params_valid {gamma: context}
+  (gamma_valid: valid_context gamma)
+  {l: list indpred_def} {p: predsym} {fs: list (string * formula)}
+  (l_in: In (inductive_def l) gamma)
+  (def_in: In (ind_def p fs) l):
+  Forall (valid_type gamma) (s_args p).
+Admitted.
+
 (*Another version with more convenient premises for us*)
 Lemma inv_aux_typed' {gamma: context} (gamma_valid: valid_context gamma)
   (l: list indpred_def)
@@ -666,22 +680,7 @@ Proof.
   apply in_inductive_ctx in Hl.
   unfold get_ind_data.
   destruct ind as [p fs].
-  (*This is actually difficult to prove, but it is derivable - 
-    separate lemma? - no, need to add*)
-  assert (Forall (valid_type gamma) (s_args p)). {
-    pose proof (valid_context_defs _ gamma_valid).
-    rewrite Forall_forall in H.
-    specialize (H _ Hlgamma).
-    simpl in H.
-    unfold indprop_valid in H.
-    destruct_all.
-    rewrite Forall_forall in H.
-    specialize (H _ Hinind).
-    simpl in H.
-    destruct fs; simpl in *.
-    (*TODO: just add this*)
-    admit.
-  }
+  assert (Hall:=indprop_params_valid gamma_valid Hlgamma Hinind).
   assert (Hp: In p (predsyms_of_indprop l)). {
     unfold predsyms_of_indprop. rewrite in_map_iff.
       exists (ind_def p fs); auto.
@@ -696,13 +695,12 @@ Proof.
     exists (predsyms_of_def (inductive_def l)); simpl; split; auto.
     rewrite in_map_iff. exists (inductive_def l); auto.
   - simpl. pose proof (in_indpred_valid_ind_form gamma_valid Hl).
-    rewrite Forall_forall in H0.
-    specialize (H0 _ Hinpfs). auto.
+    rewrite Forall_forall in H.
+    specialize (H _ Hinpfs). auto.
   - simpl. pose proof (in_indpred_valid gamma_valid Hl).
-    rewrite Forall_map, Forall_forall in H0.
-    specialize (H0 _ Hinpfs).
-    rewrite Forall_forall in H; auto.
-Admitted.
+    rewrite Forall_map, Forall_forall in H.
+    specialize (H _ Hinpfs). auto.
+Qed.
 
 (*TODO: name this?*)
 (*No, we do not want to prove closed. Can we do without?*)
@@ -906,6 +904,64 @@ Proof.
     + apply IHts. lia.
 Qed. 
 
+(*Version with typing lemmas, specialized to fun or predsym args*)
+Lemma arg_list_hnth_eq (s: fpsym) {i: nat} {args: list vty}
+  (Hi: i < length args) vt:
+  v_subst vt (ty_subst (s_params s) (map vty_var (s_params s)) (nth i args vty_int)) =
+  nth i (ty_subst_list_s (s_params s) (map (v_subst vt) (map vty_var (s_params s)))
+    args) s_int.
+Proof.
+  unfold ty_subst_list_s.
+  rewrite map_nth_inbound with(d2:=vty_int);
+  auto.
+  apply funsym_subst_eq.
+  apply s_params_Nodup. rewrite map_length; auto.
+Qed.
+
+Lemma arg_list_hnth_ty {gamma} {s: fpsym} {ts: list term} 
+{vs: list vty} {args: list vty}
+(Hlents : length ts = length args)
+(Hall : Forall
+  (fun x : term * vty => term_has_type gamma (fst x) (snd x))
+  (combine ts (map (ty_subst (s_params s) vs) args)))
+{i: nat} (Hi: i < length args): 
+term_has_type gamma (nth i ts tm_d) (ty_subst (s_params s) vs (nth i args vty_int)).
+Proof.
+  rewrite Forall_forall in Hall.
+  apply (Hall (nth i ts tm_d, ty_subst (s_params s) vs (nth i args vty_int))).
+  rewrite in_combine_iff; [| rewrite map_length; auto].
+  exists i. split; try lia. intros.
+  f_equal; [apply nth_indep |]; try lia.
+  rewrite map_nth_inbound with (d2:=vty_int); auto.
+Qed.
+
+(*When our params are [map vty_var (s_params p)]*)
+Lemma get_arg_list_hnth_unif {gamma: context} 
+(pd : pi_dom) (v: val_typevar)
+(s: fpsym) (ts: list term) 
+(reps: forall (t: term) (ty: vty),
+  term_has_type gamma t ty ->
+  domain (dom_aux pd) (v_subst v ty))
+(Hreps: forall (t: term) (ty: vty)
+  (Hty1 Hty2: term_has_type gamma t ty),
+  reps t ty Hty1 = reps t ty Hty2)
+{args: list vty}
+(Hlents: length ts = length args)
+(Hlenvs: length (map vty_var (s_params s))  = length (s_params s))
+(Hall: Forall (fun x => term_has_type gamma (fst x) (snd x))
+  (combine ts (map (ty_subst (s_params s) (map vty_var (s_params s))) args)))
+(i: nat)
+(Hi: i < length args):
+hnth i
+  (get_arg_list pd v s (map vty_var (s_params s)) ts reps Hlents Hlenvs Hall) s_int (dom_int pd) =
+  dom_cast (dom_aux pd) (arg_list_hnth_eq s Hi v)
+  (reps (nth i ts tm_d) (ty_subst (s_params s) 
+    (map vty_var (s_params s)) (nth i args vty_int))
+  (arg_list_hnth_ty Hlents Hall Hi)).
+Proof.
+  apply get_arg_list_hnth; auto.
+Qed. 
+
 (*Generate an hlist of a given type from a function*)
 Fixpoint gen_hlist {A: Type} (f: A -> Type) (g: forall (a: A), f a)
   (l: list A) :
@@ -1029,9 +1085,6 @@ Qed.
 
 (*We can reason about [descend] in terms of
   [indpred_decomp]*)
-Print indpred_transform.
-Search indpred_transform.
-Print fforalls.
 
 Definition fexists (vs: list vsymbol) (f: formula) :=
   fold_right (fun x acc => Fquant Texists x acc) f vs.
@@ -2137,7 +2190,6 @@ Proof.
   induction Hind; inversion Hty; subst; simpl in *; auto.
 Qed.
 
-Search substi_multi_let nth.
 (*
 Lemma substi_multi_let_nth {gamma: context}
 (gamma_valid: valid_context gamma) (pd: pi_dom)
@@ -2219,6 +2271,360 @@ Proof.
   - intros. apply (Hagree2 t0); auto.
 Qed.
 
+(*Disjoint lists*)
+(*TODO: name clash with pat match*)
+Section Disj.
+Context {A: Type}.
+Definition disj (l1 l2: list A) : Prop :=
+  forall x, ~ (In x l1 /\ In x l2).
+Lemma disj_l12_iff (l1 l2: list A):
+  disj l1 l2 <-> (forall x, In x l1 -> ~ In x l2).
+Proof.
+  unfold disj.
+  split; intros.
+  - intro C. apply (H _ (conj H0 C)).
+  - intro C. destruct C.
+    apply (H _ H0 H1).
+Qed.
+
+Lemma disj_l12 {l1 l2: list A}:
+  disj l1 l2 -> (forall x, In x l1 -> ~ In x l2).
+Proof.
+  apply disj_l12_iff.
+Qed.
+
+Lemma disj_comm (l1 l2: list A):
+  disj l1 l2 <-> disj l2 l1.
+Proof.
+  unfold disj. split; intros; rewrite and_comm; auto.
+Qed.
+
+Lemma disj_l21_iff (l1 l2: list A):
+  disj l1 l2 <-> (forall x, In x l2 -> ~ In x l1).
+Proof.
+  rewrite disj_comm. apply disj_l12_iff.
+Qed.
+
+Lemma disj_l21 {l1 l2: list A}:
+  disj l1 l2 -> (forall x, In x l2 -> ~ In x l1).
+Proof.
+  apply disj_l21_iff.
+Qed.
+
+Lemma disj_sublist {l1 l2 l3: list A}:
+  disj l1 l2 ->
+  sublist l3 l2 ->
+  disj l1 l3.
+Proof.
+  unfold disj, sublist; intros Hsub Hdisj x [Hinx1 Hinx2].
+  apply (Hsub x); split; auto.
+Qed.
+
+End Disj.
+
+(*More lemmas about decomp*)
+Lemma tup_2_fv (f: formula):
+  forall (t: term) (x: vsymbol), 
+  In t (map snd (tup_2 (indpred_decomp f))) ->
+  In x (tm_fv t) ->
+  In x (fmla_fv f ++ fmla_bnd f).
+Proof.
+  intros t x. rewrite in_app_iff. revert f.
+  apply (formula_ind (fun _ => True)
+    (fun f => In t (map snd (tup_2 (indpred_decomp f))) ->
+    In x (tm_fv t) -> In x (fmla_fv f) \/ In x (fmla_bnd f)));
+  auto; simpl; intros; try contradiction.
+  - destruct q; try contradiction.
+    simpl in H0.
+    apply H in H0; auto. simpl_set. vsym_eq x v. destruct_all; auto.
+  - destruct b; try contradiction.
+    rewrite in_app_iff. simpl_set. simpl in H1.
+    apply H0 in H1; auto. destruct_all; auto.
+  - simpl_set. rewrite in_app_iff. destruct H1; subst; auto.
+    apply H0 in H1; auto.
+    vsym_eq x v. destruct_all; auto.
+Qed.
+
+Lemma tup_2_fv_closed (f: formula):
+  closed_formula f ->
+  forall (t: term) (x: vsymbol), 
+  In t (map snd (tup_2 (indpred_decomp f))) ->
+  In x (tm_fv t) ->
+  In x (fmla_bnd f).
+Proof.
+  unfold closed_formula. rewrite null_nil. intros.
+  pose proof (tup_2_fv f t x H0 H1).
+  rewrite H in H2. auto.
+Qed.
+
+Lemma tup_4_fv (f: formula):
+  forall (x: vsymbol),
+  In x (fmla_fv (tup_4 (indpred_decomp f))) ->
+  In x (fmla_fv f ++ fmla_bnd f).
+Proof.
+  intros x. rewrite in_app_iff.
+  revert f.
+  apply (formula_ind (fun _ => True)
+    (fun f => In x (fmla_fv (tup_4 (indpred_decomp f))) -> In x (fmla_fv f) \/ In x (fmla_bnd f)));
+  auto; simpl; intros; simpl_set.
+  - destruct q; simpl in *; simpl_set; auto.
+    apply H in H0. vsym_eq x v. destruct_all; auto.
+  - destruct b; simpl in *; simpl_set; auto.
+    rewrite in_app_iff.
+    apply H0 in H1; destruct_all; auto.
+  - apply H0 in H1. vsym_eq x v. rewrite in_app_iff. 
+    destruct H1; auto.
+Qed.
+
+Lemma tup_4_fv_closed (f: formula):
+  closed_formula f ->
+  forall(x: vsymbol), 
+  In x (fmla_fv (tup_4 (indpred_decomp f))) ->
+  In x (fmla_bnd f).
+Proof.
+  unfold closed_formula. rewrite null_nil. intros.
+  pose proof (tup_4_fv f x H0).
+  rewrite H in H1. auto.
+Qed.
+
+(*(tm_bnd (tup_1)) is NoDup if bnd is NoDup*)
+Lemma tup_1_NoDup (f: formula):
+  NoDup (fmla_bnd f) ->
+  NoDup (tup_1 (indpred_decomp f)).
+Proof.
+  revert f.
+  apply (formula_ind (fun _ => True) (fun f =>
+  NoDup (fmla_bnd f) -> NoDup (tup_1 (indpred_decomp f))));
+  auto; simpl; intros; try solve[constructor].
+  - inversion H0; subst.
+    specialize (H H4). destruct q; try constructor; auto.
+    intros Hv.
+    apply indpred_decomp_bound in Hv.
+    contradiction.
+  - rewrite NoDup_app_iff in H1.
+    destruct_all.
+    destruct b; simpl; auto; constructor.
+  - inversion H1; subst.
+    rewrite NoDup_app_iff in H5.
+    destruct_all.
+    auto.
+Qed.
+
+Lemma tup_2_NoDup (f: formula):
+  NoDup (fmla_bnd f) ->
+  NoDup (map fst (tup_2 (indpred_decomp f))).
+Proof.
+  revert f.
+  apply (formula_ind (fun _ => True) (fun f =>
+  NoDup (fmla_bnd f) -> NoDup (map fst (tup_2 (indpred_decomp f)))));
+  auto; simpl; intros; try solve[constructor].
+  - inversion H0; subst. destruct q; simpl; auto; constructor.
+  - rewrite NoDup_app_iff in H1; destruct_all.
+    destruct b; simpl; auto; constructor.
+  - inversion H1; subst.
+    rewrite NoDup_app_iff in H5; destruct_all.
+    constructor; auto.
+    intro C.
+    rewrite in_map_iff in C.
+    destruct C as [x [Hv Hinx]]; subst.
+    apply indpred_decomp_bound in Hinx.
+    apply H4. rewrite in_app_iff; auto.
+Qed.
+
+Lemma alpha_closed (f1 f2: formula):
+  a_equiv_f f1 f2 ->
+  closed_formula f1 = closed_formula f2.
+Proof.
+  intros.
+  unfold closed_formula.
+  apply is_true_eq.
+  rewrite !null_nil.
+  pose proof (alpha_equiv_f_fv f1 f2 H).
+  split; intros Hfv; rewrite Hfv in H0; simpl in H0.
+  - destruct (fmla_fv f2); auto. exfalso. apply (H0 v); simpl; auto.
+  - destruct (fmla_fv f1); auto. exfalso. apply (H0 v); simpl; auto.
+Qed.
+
+(*TODO: move to Alpha*)
+Lemma a_convert_all_f_bnd_NoDup f vs:
+NoDup (fmla_bnd (a_convert_all_f f vs)).
+Proof.
+  unfold a_convert_all_f.
+  apply alpha_f_aux_bnd.
+  apply gen_strs_nodup.
+  rewrite gen_strs_length. auto.
+Qed.
+
+Lemma a_convert_all_f_bnd f vs:
+  disj vs (fmla_bnd (a_convert_all_f f vs)).
+Proof.
+  unfold disj. intros x [Hinx1 Hinx2].
+  apply alpha_f_aux_bnd in Hinx2.
+  - apply gen_strs_notin in Hinx2.
+    rewrite !in_app_iff in Hinx2. not_or Hinx.
+    contradiction.
+  - apply gen_strs_nodup.
+  - rewrite gen_strs_length; auto.
+Qed.
+
+(*TODO: just putting a bunch of lemmas, figure out organization*)
+Lemma vt_with_args_eq (vt: val_typevar) (params: list typevar):
+  NoDup params ->
+  vt_with_args vt params (map vt params) = vt.
+Proof.
+  intros Hnodup.
+  apply functional_extensionality_dep; intros.
+  destruct (in_dec typevar_eq_dec x params).
+  - destruct (In_nth _ _ EmptyString i) as [n [Hn Hx]]; subst.
+    rewrite vt_with_args_nth; auto.
+    rewrite map_nth_inbound with(d2:=EmptyString); auto.
+    rewrite map_length; auto.
+  - apply vt_with_args_notin; auto.
+Qed.
+(*The [hlist]s (essentially the IH) that we need
+  for the inversion lemma*)
+Lemma inv_Ps_ty {gamma: context} (gamma_valid: valid_context gamma)
+  {l: list indpred_def} (l_in: In (inductive_def l) gamma)
+  (p: predsym) (fs: list (string * formula))
+  (Hinpfs: In (p, fs) (map get_ind_data l)):
+  formula_typed gamma
+    (map_join_left Ftrue
+      (exi (create_vsymbols (concat (map fmla_bnd (map snd fs))) 
+      (s_args p))) t_or fs).
+Proof.
+  intros.
+  pose proof (inv_aux_typed' gamma_valid l l_in (p, fs) Hinpfs).
+  simpl in H.
+  apply fforalls_typed_inv in H.
+  destruct H.
+  inversion H; auto.
+Qed.
+
+Lemma inv_Ps_cast (vt: val_typevar) (p: fpsym) (fs: list (string * formula)) srts:
+  srts =  (map (v_subst vt) (map vty_var (s_params p))) ->
+  sym_sigma_args p srts =
+  map (v_subst vt)
+    (map snd (create_vsymbols (concat (map fmla_bnd (map snd fs))) (s_args p))).
+Proof.
+  intros. subst. unfold create_vsymbols.
+  rewrite map_snd_combine; [|rewrite gen_strs_length; auto].
+  apply sym_sigma_args_params.
+Qed.
+
+Definition inv_Ps {gamma} (gamma_valid: valid_context gamma) 
+  (pd: pi_dom) (vt: val_typevar)
+  (vv: val_vars pd vt)
+  (pf: pi_funpred gamma_valid pd) {l: list indpred_def}
+  (l_in: In (inductive_def l) gamma) : 
+
+  hlist (fun p' : predsym =>
+  forall srts : list sort,
+  arg_list (domain (dom_aux pd)) (sym_sigma_args p' srts) -> bool)
+  (map fst (get_indpred l)) :=
+
+  gen_hlist (fun p' : predsym =>
+    forall srts : list sort,
+    arg_list (domain (dom_aux pd)) (sym_sigma_args p' srts) -> bool)
+    (fun (p': predsym) =>
+      fun (srts: list sort) (a: arg_list (domain (dom_aux pd)) (sym_sigma_args p' srts)) =>
+      (*Body of function*)
+      (*We need srts to be correct*)
+      match (list_eq_dec sort_eq_dec srts 
+        (map (v_subst vt) (map vty_var (s_params p')))) with
+      | left Heq => 
+          (*Get the list of formulas for this predsym*)
+          let fs := match get_assoc_list predsym_eq_dec (map get_ind_data l) p' with
+          | Some l => l
+          | None => nil
+          end in
+          (*Not very elegant, but check to see if this is
+            in the indpred list. This check will
+            always be true*)
+          match (in_dec (tuple_eq_dec predsym_eq_dec (list_eq_dec 
+            (tuple_eq_dec string_dec formula_eq_dec))) 
+            (p', fs) (map get_ind_data l)) with
+          | left Hin => 
+              formula_rep gamma_valid pd vt pf
+              (substi_mult' vt vv
+              (create_vsymbols (concat (map fmla_bnd (map snd fs))) (s_args p')) 
+                (cast_arg_list (inv_Ps_cast vt p' fs srts Heq) (*cast lemma*)  a))
+              (map_join_left Ftrue
+              (exi (create_vsymbols (concat (map fmla_bnd (map snd fs))) (s_args p'))) t_or fs)
+              (inv_Ps_ty gamma_valid l_in p' fs Hin) (*typing proof*)
+          | right Hnotin => false
+          end
+      | right Hneq => false
+      end) (map fst (get_indpred l)).
+
+Lemma predsyms_of_indprop_Nodup {gamma} (gamma_valid: valid_context gamma)
+  (l: list indpred_def) (l_in: In (inductive_def l) gamma):
+  NoDup (predsyms_of_indprop l).
+Proof.
+  apply valid_context_wf in gamma_valid.
+  apply wf_context_sig_Nodup in gamma_valid.
+  destruct gamma_valid as [_ [Hn _ ]].
+  unfold sig_p in Hn.
+  rewrite NoDup_concat_iff in Hn.
+  destruct Hn as [Hn _]; apply Hn.
+  rewrite in_map_iff. exists (inductive_def l); auto.
+Qed.
+
+(*General results about indprops*)
+Lemma constr_valid_ind_form {gamma}
+  (gamma_valid: valid_context gamma) {l p fs f}
+  (l_in: In (inductive_def l) gamma)
+  (p_in: In (p, fs) (get_indpred l))
+  (f_in: In f fs):
+  valid_ind_form p f.
+Proof.
+  apply in_inductive_ctx in l_in.
+  pose proof (in_indpred_valid_ind_form gamma_valid l_in).
+  rewrite Forall_forall in H.
+  specialize (H  _ p_in).
+  rewrite Forall_forall in H; apply H; auto.
+Qed.
+
+Lemma constr_typed {gamma}
+  (gamma_valid: valid_context gamma) {l p fs f}
+  (l_in: In (inductive_def l) gamma)
+  (p_in: In (p, fs) (get_indpred l))
+  (f_in: In f fs):
+  formula_typed gamma f.
+Proof.
+  apply in_inductive_ctx in l_in.
+  apply (indprop_fmla_valid gamma_valid l_in p_in f_in).
+Qed.
+
+Lemma constr_pos {gamma}
+  (gamma_valid: valid_context gamma) {l p fs f}
+  (l_in: In (inductive_def l) gamma)
+  (p_in: In (p, fs) (get_indpred l))
+  (f_in: In f fs):
+  ind_positive (map fst (get_indpred l)) f.
+Proof.
+  apply in_inductive_ctx in l_in.
+  pose proof (in_indpred_positive gamma_valid l_in).
+  rewrite Forall_map, Forall_forall in H.
+  specialize (H _ p_in). simpl in H.
+  rewrite Forall_forall in H.
+  specialize (H _ f_in); auto.
+Qed.
+
+Lemma constr_closed {gamma}
+  (gamma_valid: valid_context gamma) {l p fs f}
+  (l_in: In (inductive_def l) gamma)
+  (p_in: In (p, fs) (get_indpred l))
+  (f_in: In f fs):
+  closed_formula f.
+Proof.
+  apply in_inductive_ctx in l_in.
+  pose proof (in_indpred_closed gamma_valid l_in).
+  rewrite Forall_map in H.
+  rewrite Forall_forall in H.
+  specialize (H _ p_in).
+  simpl in H. rewrite Forall_forall in H.
+  apply H; auto.
+Qed.
 
 Theorem gen_axioms_sound : sound_trans (single_trans gen_axioms).
 Proof.
@@ -2228,7 +2634,8 @@ Proof.
     (*Now the hard part - show log conseq*)
     unfold log_conseq_gen.
     intros.
-    destruct pf_full as [Hrecfun [Hrecpred [Hindc Hindlf]]].
+    assert (Hfull:=pf_full).
+    destruct Hfull as [_ [_ [Hindc Hindlf]]].
     unfold satisfies.
     intros.
     (*First, get more info about fmla*)
@@ -2256,7 +2663,7 @@ Proof.
       (*Now, use the contruct fact*)
       assert (Hcon := Hindc).
       specialize (Hcon (get_indpred l) (in_inductive_ctx _ _ Hind) p
-        (map snd l0)).
+        (map snd l0)). clear Hindc Hindlf.
       assert (p_in: In (p, map snd l0) (get_indpred l)). {
         unfold get_indpred. rewrite in_map_iff.
         exists (ind_def p l0); auto.
@@ -2271,23 +2678,23 @@ Proof.
         val_typevar*)
       assert (Hnodup: NoDup (s_params p)) by
         (apply s_params_Nodup).
-       (*Let us prove that these val_typevars are really equal*)
-      assert (vt = (vt_with_args vt (s_params p) (map vt (s_params p)))). {
-        apply functional_extensionality_dep; intros.
-        symmetry.
-        destruct (in_dec typevar_eq_dec x (s_params p)).
-        -- destruct (In_nth _ _ EmptyString i) as [n [Hn Hx]]; subst.
-          rewrite vt_with_args_nth; auto.
-          rewrite map_nth_inbound with(d2:=EmptyString); auto.
-        -- apply vt_with_args_notin; auto.
-      }
-      rewrite <- H in Hcon.
+      (*Simplify val_typevar*)
+      rewrite (vt_with_args_eq vt (s_params p) Hnodup) in Hcon.
       specialize (Hcon vv (snd ax)).
       assert (f_in: In (snd ax) (map snd l0)).
       { rewrite in_map_iff. exists ax; auto. }
       specialize (Hcon f_in).
       erewrite fmla_rep_irrel. apply Hcon.
     + (*Inversion axiom case (much harder)*)
+      (*A lemma we will need*)
+      assert (Hnodup: NoDup (map fst (map get_ind_data l))). {
+        replace (map fst (map get_ind_data l)) with
+          (predsyms_of_indprop l).
+        - apply (predsyms_of_indprop_Nodup gamma_valid); auto.
+        - unfold predsyms_of_indprop.
+          rewrite !map_map.
+          apply map_ext; intros [x1 x2]; auto.
+      }
       (*First, simplify In*)
       rewrite in_map_iff in Hinax.
       destruct Hinax as [ind [Hax Hinind]]; subst.
@@ -2296,19 +2703,18 @@ Proof.
       destruct Hinind as [ind_d [Heq Hind]]; subst.
       destruct ind_d. simpl in *.
       (*We need this and it is much nicer to have it opaque*)
-      assert (Hty1: formula_typed (task_gamma t)
-      (Fbinop Timplies
-         (Fpred p (map vty_var (s_params p))
-            (map Tvar (create_vsymbols (concat (map fmla_bnd (map snd l0))) (s_args p))))
-         (map_join_left Ftrue
-            (exi (create_vsymbols (concat (map fmla_bnd (map snd l0))) (s_args p))) t_or l0))).
-      { exact (proj1' (fforalls_typed_inv _ _ Hty)). }
+      assert (Hty1:=(proj1'(fforalls_typed_inv _ _ Hty))).
       (*We can simplify the fforalls and implies*)
       erewrite fmla_rep_irrel.
       rewrite fforalls_rep'.
       Unshelve.
       2: { exact Hty1. }
-      2: { (*same as before, need separate lemma after assumption*) admit. }
+      2: {
+        rewrite <- Forall_map.
+        unfold create_vsymbols.
+        rewrite map_snd_combine; [| rewrite gen_strs_length; auto].
+        apply (indprop_params_valid gamma_valid l_in Hind).
+      }
       rewrite simpl_all_dec.
       intros h.
       simpl_rep_full. rewrite bool_of_binop_impl, simpl_all_dec.
@@ -2328,10 +2734,8 @@ Proof.
       length (s_params p)) by (rewrite !map_length; auto).
       specialize (Hleast Hparamslen).
       (*Some simplification on the [pred_arg_list] and h we have:*)
-      assert (Hsigma: sym_sigma_args p (map (v_subst vt) (map vty_var (s_params p))) =
-        map (v_subst vt) (s_args p)).
-      { apply sym_sigma_args_params. }
-      assert (Hmapsnd:  (map snd (create_vsymbols (concat (map fmla_bnd (map snd l0))) (s_args p)))
+      assert (Hsigma:=sym_sigma_args_params vt p).
+      assert (Hmapsnd: (map snd (create_vsymbols (concat (map fmla_bnd (map snd l0))) (s_args p)))
         = s_args p).
       {
         unfold create_vsymbols. rewrite map_snd_combine; auto.
@@ -2359,37 +2763,7 @@ Proof.
         assert (Hlencreate: length (create_vsymbols (concat (map fmla_bnd (map snd l0))) (s_args p))=
           length (s_args p)).
         { rewrite <- Hmapsnd at 2. rewrite map_length; auto. }
-        (*2 lemmas we need for [get_arg_list_hnth]*)
-        assert (Heq: v_subst vt
-          (ty_subst (s_params p) (map vty_var (s_params p)) (nth i (s_args p) vty_int)) =
-        nth i
-          (ty_subst_list_s (s_params p) (map (v_subst vt) (map vty_var (s_params p)))
-            (s_args p)) s_int).
-        {
-          unfold ty_subst_list_s. rewrite map_nth_inbound with(d2:=vty_int);
-          auto. apply funsym_subst_eq; auto.
-          apply s_params_Nodup. rewrite map_length; auto.
-        } 
-        assert (Hty2: term_has_type (task_gamma t)
-        (nth i (map Tvar (create_vsymbols (concat (map fmla_bnd (map snd l0))) (s_args p)))
-           tm_d)
-        (ty_subst (s_params p) (map vty_var (s_params p)) (nth i (s_args p) vty_int))).
-        {
-          rewrite map_nth_inbound with(d2:=vs_d); try lia.
-          unfold create_vsymbols. 
-          unfold vs_d, vsymbol. rewrite combine_nth;
-          [| rewrite gen_strs_length; auto].
-          apply T_Var'.  (*again*) admit.
-          simpl.
-          symmetry. apply ty_subst_params_id.
-          intros. (*TODO: definitely separate lemma*)
-          destruct p; simpl in *.
-          destruct p_sym; simpl in *.
-          assert (Hwf:=s_args_wf).
-          apply check_args_prop with(x:=nth i s_args vty_int) 
-          in Hwf; auto. apply nth_In; auto.
-        }
-        erewrite (get_arg_list_hnth pd vt p (map vty_var (s_params p))
+        rewrite (get_arg_list_hnth_unif pd vt p
         (map Tvar (create_vsymbols (concat (map fmla_bnd (map snd l0))) 
           (s_args p)))
           (term_rep gamma_valid pd vt pf
@@ -2397,8 +2771,9 @@ Proof.
              (create_vsymbols (concat (map fmla_bnd (map snd l0))) (s_args p)) h))
           (ltac:(intros; apply term_rep_irrel))
              (proj1' (pred_val_inv (proj1' (typed_binop_inv Hty1)))))
-        with(Heq:=Heq)(Hty:=Hty2); auto.
-        revert Hty2.
+        with(Hi:=Hi).
+        generalize dependent (arg_list_hnth_ty (proj1' (pred_val_inv (proj1' (typed_binop_inv Hty1))))
+        (proj2' (proj2' (pred_val_inv (proj1' (typed_binop_inv Hty1))))) Hi).
         rewrite map_nth_inbound with (d2:=vs_d); try lia.
         intros.
         simpl_rep_full. unfold var_to_dom.
@@ -2417,18 +2792,13 @@ Proof.
       (*Now we will only work with h*)
       specialize (Hleast (cast_arg_list (eq_trans (f_equal (map (v_subst vt)) Hmapsnd) (eq_sym Hsigma))
       h) vt).
-      (*Now we prove equality of vt (like constr case)*)
+      (*Again, simplify val_typevar*)
       assert (vt = (vt_with_args vt (s_params p)
       (map (v_subst vt) (map vty_var (s_params p))))). {
-        apply functional_extensionality_dep; intros.
-        symmetry.
-        destruct (in_dec typevar_eq_dec x (s_params p)).
-        -- destruct (In_nth _ _ EmptyString i) as [n [Hn Hx]]; subst.
-          rewrite vt_with_args_nth; auto; [|apply s_params_Nodup].
-          rewrite !map_map.
-          rewrite map_nth_inbound with(d2:=EmptyString); auto.
-          apply sort_inj; simpl. reflexivity.
-        -- apply vt_with_args_notin; auto.
+        rewrite <- (vt_with_args_eq vt (s_params p) (s_params_Nodup _)) at 1.
+        f_equal.
+        rewrite !map_map.
+        apply map_ext. intros. apply sort_inj; auto.
       }
       rewrite <- H in Hleast. clear H.
       specialize (Hleast vv).
@@ -2436,70 +2806,7 @@ Proof.
         we will substitute. This is actually not too bad,
         we just interpret the corresponding inversion lemma
         with the arg_list argument for our variables*)
-      (*Lemmas we need (TODO: combine with above)*)
-      assert (Hacast: forall p' (fs: list (string * formula)) srts,
-      srts =  (map (v_subst vt) (map vty_var (s_params p'))) ->
-      sym_sigma_args p' srts =
-      map (v_subst vt)
-        (map snd (create_vsymbols (concat (map fmla_bnd (map snd fs))) (s_args p')))).
-      {
-        intros. subst. unfold create_vsymbols.
-        rewrite map_snd_combine; [|rewrite gen_strs_length; auto].
-        apply sym_sigma_args_params.
-      }
-      assert (Hallty': forall (p': predsym) (fs: list (string * formula))
-        (Hinpfs: In (p', fs) (map get_ind_data l)),
-      formula_typed (task_gamma t)
-      (map_join_left Ftrue
-         (exi (create_vsymbols (concat (map fmla_bnd (map snd fs))) 
-         (s_args p'))) t_or fs)).
-      {
-        intros.
-        epose proof (inv_aux_typed' gamma_valid l l_in (p', fs) Hinpfs).
-        simpl in H.
-        apply fforalls_typed_inv in H.
-        destruct H.
-        inversion H; auto.
-      }
-     (*Finally, we build Ps. The definition is complicated, but
-     the idea is that we just evaluate the inversion lemma for the
-     given predsym with the valuation for the free variables as
-     the inputted arg_list*)
-      set (Ps:=gen_hlist (fun p' : predsym =>
-        forall srts : list sort,
-        arg_list (domain (dom_aux pd)) (sym_sigma_args p' srts) -> bool)
-        (fun (p': predsym) =>
-          fun (srts: list sort) (a: arg_list (domain (dom_aux pd)) (sym_sigma_args p' srts)) =>
-          (*Body of function*)
-          (*We need srts to be correct*)
-          match (list_eq_dec sort_eq_dec srts 
-            (map (v_subst vt) (map vty_var (s_params p')))) with
-          | left Heq => 
-              (*Get the list of formulas for this predsym*)
-              let fs := match get_assoc_list predsym_eq_dec (map get_ind_data l) p' with
-              | Some l => l
-              | None => nil
-              end in
-              (*Not very elegant, but check to see if this is
-                in the indpred list. This check will
-                always be true*)
-              match (in_dec (tuple_eq_dec predsym_eq_dec (list_eq_dec 
-                (tuple_eq_dec string_dec formula_eq_dec))) 
-                (p', fs) (map get_ind_data l)) with
-              | left Hin => 
-                  formula_rep gamma_valid pd vt pf
-                  (substi_mult' vt vv
-                  (create_vsymbols (concat (map fmla_bnd (map snd fs))) (s_args p')) 
-                    (cast_arg_list (Hacast p' fs srts Heq) a))
-                  (map_join_left Ftrue
-                  (exi (create_vsymbols (concat (map fmla_bnd (map snd fs))) (s_args p'))) t_or fs)
-                  (Hallty' p' fs Hin) (*typing proof*)
-              | right Hnotin => false
-              end
-              (*TODO: rest - need l0 (to get)*)
-          | right Hneq => false
-          end) (map fst (get_indpred l))
-      ).
+      set (Ps:=inv_Ps gamma_valid pd vt vv pf l_in).
       specialize (Hleast Ps).
       (*Now prove that the goal matches the conclusion of Hleast*)
       match goal with
@@ -2514,7 +2821,7 @@ Proof.
       (*We have 2 goals left: show that the goal is [get_hlist_elt]
         and the main part, prove that the inversion axioms make the
         constructors true*)
-      * subst Ps. rewrite gen_hlist_get_elt.
+      * subst Ps. unfold inv_Ps. rewrite gen_hlist_get_elt.
         destruct ( list_eq_dec sort_eq_dec (map (v_subst vt) (map vty_var (s_params p)))
         (map (v_subst vt) (map vty_var (s_params p))));
         try contradiction.
@@ -2522,10 +2829,7 @@ Proof.
           unfold get_ind_data. rewrite in_map_iff.
           exists (ind_def p l0); auto.
         }
-        (*TODO: prove in general*)
-        assert (Hnodup: NoDup (map fst (map get_ind_data l))). { admit. }
         rewrite get_assoc_list_nodup with(y:=l0); auto.
-        simpl.
         destruct (in_dec
         (tuple_eq_dec predsym_eq_dec
            (list_eq_dec (tuple_eq_dec string_dec formula_eq_dec))) (
@@ -2534,7 +2838,7 @@ Proof.
         rewrite cast_arg_list_same.
         erewrite fmla_rep_irrel. reflexivity.
       * (*Now, finally, we are left only with the main goal*)
-        clear Heq Hparamslen Hleast H0 Hindlf Hindc Hrecpred Hrecfun Hp h.
+        clear Heq Hparamslen Hleast H0 Hindlf Hindc Hp h.
         (*TODO: prove in other lemma for sure*)
         intros fs Hform Hinfs.
         apply prove_iter_and. intros P.
@@ -2546,25 +2850,10 @@ Proof.
           First, we alpha convert to make wf*)
         rewrite in_map_iff in Hinfs.
         destruct Hinfs as [[p' fs'] [Hfs Hinfs]]; simpl in *; subst.
-        assert (Hindf: valid_ind_form p' constr).
-        {
-          apply in_inductive_ctx in l_in.
-          pose proof (in_indpred_valid_ind_form gamma_valid l_in).
-          rewrite Forall_forall in H.
-          specialize (H  _ Hinfs).
-          rewrite Forall_forall in H; apply H; auto.
-        }
-        assert (Hvalf: formula_typed (task_gamma t) constr). {
-          rewrite Forall_forall in Hform. apply Hform; auto.
-        }
-        assert (Hposf: ind_positive (map fst (get_indpred l)) constr). {
-          apply in_inductive_ctx in l_in.
-          pose proof (in_indpred_positive gamma_valid l_in).
-          rewrite Forall_map, Forall_forall in H.
-          specialize (H _ Hinfs). simpl in H.
-          rewrite Forall_forall in H.
-          specialize (H _ Hinconstrs); auto.
-        }
+        assert (Hindf:=constr_valid_ind_form gamma_valid l_in Hinfs Hinconstrs).
+        assert (Hvalf:= constr_typed gamma_valid l_in Hinfs Hinconstrs).
+        assert (Hposf:=constr_pos gamma_valid l_in Hinfs Hinconstrs).
+        (*And get the properties of the alpha-renamed version*)
         set (create_vsymbols (concat (map fmla_bnd fs)) (s_args p')) as vs.
         rewrite (Alpha.a_convert_all_f_rep gamma_valid _ _ vs).
         assert (Hinda:=(Alpha.a_convert_all_f_valid_ind_form p' constr vs Hindf)).
@@ -2590,7 +2879,6 @@ Proof.
         intros Hconstrs.
         (*Now we are at the end, which we know is p(...) under Ps.
           We must prove the inversion lemma*)
-        (*TODO: do we need an alpha version that does not change these vars?*)
         generalize dependent (proj2' (typed_binop_inv Hval2)).
         rewrite ind_form_decomp with(p:=p'); auto.
         intros Hty4.
@@ -2601,7 +2889,7 @@ Proof.
           exists (p', fs); auto.
         }
         rewrite find_apply_pred_in with(Hinp:=Hinp').
-        unfold Ps at 1.
+        unfold Ps at 1. unfold inv_Ps at 1.
         rewrite gen_hlist_get_elt.
         (*Now we simplify to undo matching*)
         destruct (list_eq_dec sort_eq_dec (map (v_subst vt) (map vty_var (s_params p')))
@@ -2618,7 +2906,6 @@ Proof.
         assert (Hinp'': In (p', fs') (map get_ind_data l)). {
           rewrite in_map_iff. exists (ind_def p' fs'); auto.
         }
-        assert (Hnodup: NoDup (map fst (map get_ind_data l))). { admit. }
         rewrite get_assoc_list_nodup with(y:=fs'); auto.
         destruct (in_dec
         (tuple_eq_dec predsym_eq_dec
@@ -2631,6 +2918,10 @@ Proof.
         unfold fs in Hincon.
         rewrite in_map_iff in Hincon.
         destruct Hincon as [[name con] [Hconstr Hincon]]; simpl in *; subst.
+        assert (Hmapvs: map snd vs = s_args p'). {
+          unfold vs, create_vsymbols. rewrite map_snd_combine; auto.
+          rewrite gen_strs_length; auto.
+        }
         assert (Halltyfs:
         Forall (formula_typed (task_gamma t))
         (map
@@ -2638,12 +2929,14 @@ Proof.
             descend vs (snd x)) fs')).
         {
           rewrite Forall_forall. intros x Hinmap.
-          (*TODO: provable but do later*) admit.
-          (*apply Hallty'.*)
-        }
-        assert (Hmapvs: map snd vs = s_args p'). {
-          unfold vs, create_vsymbols. rewrite map_snd_combine; auto.
-          rewrite gen_strs_length; auto.
+          rewrite in_map_iff in Hinmap.
+          destruct Hinmap as [t' [Hx Hint']]; subst.
+          destruct t' as [name' fmla']; simpl in *; subst.
+          assert (Hinfs': In fmla' fs).
+          { subst fs. rewrite in_map_iff. exists (name', fmla'); auto. }
+          apply descend_typed with(p:=p'); auto.
+          - apply (constr_valid_ind_form gamma_valid l_in Hinfs); auto.
+          - apply (constr_typed gamma_valid l_in Hinfs); auto.
         }
         assert (Hdesty: formula_typed (task_gamma t) (descend vs constr)).
         {
@@ -2657,40 +2950,25 @@ Proof.
         assert (Hdesaty: formula_typed (task_gamma t) (descend vs (a_convert_all_f constr vs))). {
           apply descend_typed with (p:=p'); auto.
         }
-        assert (Hnotinvs: forall x : vsymbol, In x vs -> ~ In x (fmla_bnd (a_convert_all_f constr vs))).
-        {
-          (*This should be easier by definition of a_convert_all*)
-          intros x Hinx1 Hinx2.
-          (*TODO: in Alpha, need theorem that no bound vars in l*)
-          unfold a_convert_all_f in Hinx2.
-          (*TODO: replace*)
-          apply alpha_f_aux_bnd in Hinx2.
-          - apply gen_strs_notin in Hinx2. rewrite !in_app_iff in Hinx2.
-            not_or Hinx. contradiction.
-          - apply gen_strs_nodup.
-          - apply gen_strs_length.
+        assert (Habnd_nodup:=a_convert_all_f_bnd_NoDup constr vs).
+        (*Why we need to use fresh vs and alpha convert: cannot
+          have clashes between variables or else [descend_alpha_equiv]
+          doesn't hold*)
+        assert (Hnotinvs:=a_convert_all_f_bnd constr vs).
+        assert (Hdisjvsbnd: disj vs (fmla_bnd constr)). {
+          unfold disj. intros x.
+          unfold vs, create_vsymbols. intros [Hinx1 Hinx2].
+          destruct x as [xn xty]; simpl in *.
+          apply in_combine_l in Hinx1.
+          replace xn with (fst (xn, xty)) in Hinx1 by auto.
+          apply gen_strs_notin in Hinx1.
+          apply Hinx1. rewrite in_concat. exists (fmla_bnd constr).
+          split; auto. rewrite in_map_iff. exists constr; auto.
         }
         rewrite descend_alpha_equiv with (f2:=(a_convert_all_f constr vs))(Hty2:=Hdesaty); auto.
-        (*Why we needed vs, bound, and alpha vars to be distinct:*)
-        2: {
-          unfold vs. intros x. unfold vsymbol.
-          unfold create_vsymbols.
-          rewrite in_combine_iff; rewrite gen_strs_length; auto.
-          intros [j [Hj Hx]].
-          specialize (Hx EmptyString vty_int); subst; simpl.
-          intros Hin.
-          (*Coq will not replace var using "set", we do
-            things a bit awkwardly to avoid huge var names*)
-          assert (sublist (fmla_bnd constr) (concat (map fmla_bnd fs))). {
-            apply concat_sublist. rewrite in_map_iff. exists constr; auto.
-          }
-          apply H in Hin.
-          eapply gen_strs_notin.
-          2: apply Hin. simpl. apply nth_In. rewrite gen_strs_length. auto.
-        }
-        2: {
-          apply a_convert_all_f_equiv.
-        }
+        2: apply (disj_l12 Hdisjvsbnd).
+        2: apply (disj_l12 Hnotinvs).
+        2: apply a_convert_all_f_equiv. 
         (*Now we use our [descend_rep] lemma*)
         rewrite descend_transform_equiv with(p:=p')(Hind:=Hinda)(Hty:=Htya)
         (Hvs:=Hmapvs); auto.
@@ -2720,119 +2998,138 @@ Proof.
         (*First, prove the second part*)
         bool_to_prop; split.
         2: {
+          (*Prove equality*)
           apply fold_is_true.
           rewrite iter_fand_rep.
           intros feq Hvalfeq.
           rewrite in_map2_iff with(d1:=vs_d)(d2:=tm_d).
-          - intros [j [Hj Hfeq]]; subst.
+          2: {
+            inversion Hty4; subst.
+            rewrite H5, <- Hmapvs, map_length. auto.
+          }
+          intros [j [Hj Hfeq]]; subst.
+          (*Before proving the equality, we can simplify
+            the inner interpretation to remove [interp_with_ps..]
+            because p cannot appear in the arguments*)
+          (*TODO: better method than writing whole thing*)
+          replace (pred_arg_list pd vt p' (map vty_var (s_params p'))
+          (snd (get_indprop_args (a_convert_all_f constr vs)))
+          (term_rep gamma_valid pd vt
+             (interp_with_Ps gamma_valid pd pf (map fst (get_indpred l)) Ps)
+             (substi_multi_let gamma_valid pd
+                (interp_with_Ps gamma_valid pd pf (map fst (get_indpred l)) Ps)
+                vt
+                (substi_mult' vt vv
+                   (tup_1 (indpred_decomp (a_convert_all_f constr vs))) h')
+                (tup_2 (indpred_decomp (a_convert_all_f constr vs))) Halltup2))
+            Hty4) with
+            (pred_arg_list pd vt p' (map vty_var (s_params p'))
+                  (snd (get_indprop_args (a_convert_all_f constr vs)))
+                  (term_rep gamma_valid pd vt pf
+                      (substi_multi_let gamma_valid pd pf vt
+                        (substi_mult' vt vv
+                            (tup_1 (indpred_decomp (a_convert_all_f constr vs))) h')
+                        (tup_2 (indpred_decomp (a_convert_all_f constr vs))) Halltup2))
+                  Hty4).
+            2: {
+              (*Idea: p cannot appear in any of the a 
+                for p(a) at end of constr, nor in any of the
+                let bindings, so we can change interp and val*)
+              apply get_arg_list_ext; auto. intros.
+              erewrite tm_change_pf.
+              erewrite tm_change_vv.
+              apply term_rep_irrel.
+              - (*P does not appear in any of the terms bound in the lets*) 
+                intros. erewrite substi_mult_notin_eq with (ps:=map fst (get_indpred l)). 
+                reflexivity.
+                + apply indpred_decomp_let_notin.
+                  auto.
+                + intros. simpl. rewrite find_apply_pred_notin; auto.
+                + auto.
+              - (*and does not appear in a*) 
+                intros. simpl. rewrite find_apply_pred_notin; auto.
+                intro C.
+                revert H0.
+                apply (get_indprop_args_pos  (map fst (get_indpred l))
+                  (a_convert_all_f constr vs) Hposa Hinda); auto.
+                apply nth_In; auto.
+              - auto.
+            }
+            (*Now we simplify the equality*)
             simpl_rep_full.
             rewrite simpl_all_dec.
-            (*Now prove that the equalities are correct*)
-            assert ((ty_var_inv (proj1' (typed_eq_inv Hvalfeq))) = eq_refl).
-            apply UIP_dec. apply vty_eq_dec.
-            rewrite H; unfold dom_cast; simpl.
+            (*Now, prove that vs, tup_1, and tup_2 consist of
+              completely disjoint variables. TODO: maybe need elsewhere*)
+            assert (Hdisj1: disj vs (tup_1 (indpred_decomp (a_convert_all_f constr vs)))).
+            {
+              apply (disj_sublist Hnotinvs). intros x. 
+              apply indpred_decomp_bound.
+            }
+            assert (Hdisj2: disj vs (map fst (tup_2 (indpred_decomp (a_convert_all_f constr vs))))).
+            {
+              apply (disj_sublist Hnotinvs). intros x Hinx.
+              rewrite in_map_iff in Hinx.
+              destruct Hinx as [y [Hx Hiny]]; subst.
+              apply indpred_decomp_bound in Hiny; auto.
+            }
+            (*First, simplify LHS. This means that we 
+              show that (nth j vs) is not in (tup_2) or (tup_1),
+              so we can find the jth element of [a]; this is the interpretation*)
             unfold var_to_dom.
-            (*Simplify LHS*)
             rewrite substi_multi_let_notin.
             2: {
-              intro C. rewrite in_map_iff in C.
-              destruct C as [[vs' t'] [Hvs Hint]]; simpl in *; subst.
-              apply indpred_decomp_bound in Hint.
-              simpl in Hint.
-              apply (Hnotinvs (nth j vs vs_d)); auto.
-              apply nth_In; auto. 
+              apply (disj_l12 Hdisj2). apply nth_In; auto.
             }
             rewrite substi_mult_notin.
             2: {
-              intro C. apply indpred_decomp_bound in C.
-              apply (Hnotinvs (nth j vs vs_d)); auto.
-              apply nth_In; auto. 
+              apply (disj_l12 Hdisj1). apply nth_In; auto.
             }
-            assert (Hn: NoDup vs).
-            {
-              unfold vs, create_vsymbols.
+            assert (Hn: NoDup vs). {
+              unfold vs. unfold create_vsymbols.
               apply NoDup_combine_l.
               apply gen_strs_nodup.
             }
+            (*Now we convert this to the nth of [a]*)
             rewrite substi_mult_nth' with(Hi:=Hj); auto.
             rewrite hnth_cast_arg_list.
-            unfold pred_arg_list.
+            unfold pred_arg_list at 1.
             assert (Hj': j < Datatypes.length (s_args p')).
             {
               rewrite <- Hmapvs; rewrite map_length; auto.
             }
-            (*Need lemmas for [get_arg_list_hnth]*)
-            assert (Heq: v_subst vt
-              (ty_subst (s_params p') (map vty_var (s_params p')) (nth j (s_args p') vty_int)) =
-            nth j
-              (ty_subst_list_s (s_params p') (map (v_subst vt) (map vty_var (s_params p')))
-                (s_args p')) s_int).
-            {
-              unfold ty_subst_list_s. rewrite map_nth_inbound with(d2:=vty_int);
-              auto. apply funsym_subst_eq; auto.
-              apply s_params_Nodup. rewrite map_length; auto.
-            } 
-            assert (Hty2: term_has_type (task_gamma t)
-            (nth j (snd (get_indprop_args (a_convert_all_f constr vs))) tm_d)
-            (ty_subst (s_params p') (map vty_var (s_params p')) (nth j (s_args p') vty_int))).
-            {
-              inversion Hvalfeq; subst.
-              rewrite ty_subst_params_id; auto.
-              assert (Hjth: nth j (s_args p') vty_int = snd (nth j vs vs_d)).
-              {
-                unfold vs, create_vsymbols, vsymbol. unfold vs_d. 
-                rewrite combine_nth; [|rewrite gen_strs_length]; simpl; auto.
-              }
-              rewrite Hjth; auto.
-              (*TODO: LEMMA!*)
-              intros.
-              destruct p'. destruct p_sym.
-              simpl in *.
-              assert (Hwf:=s_args_wf).
-              apply check_args_prop with (x:=(nth j s_args vty_int)) in Hwf;
-              auto.
-              apply nth_In; auto.
-            }
-            erewrite (get_arg_list_hnth pd vt p' (map vty_var (s_params p'))
+            erewrite (get_arg_list_hnth_unif pd vt p'
             (snd (get_indprop_args (a_convert_all_f constr vs)))
-            (term_rep gamma_valid pd vt
-              (interp_with_Ps gamma_valid pd pf (map fst (get_indpred l)) Ps)
-              (substi_multi_let gamma_valid pd
-                (interp_with_Ps gamma_valid pd pf (map fst (get_indpred l)) Ps) vt
-                (substi_mult' vt vv
-                    (tup_1 (indpred_decomp (a_convert_all_f constr vs))) h')
-                (tup_2 (indpred_decomp (a_convert_all_f constr vs))) Halltup2))
+            (term_rep gamma_valid pd vt pf
+                 (substi_multi_let gamma_valid pd pf vt
+                    (substi_mult' vt vv
+                       (tup_1 (indpred_decomp (a_convert_all_f constr vs))) h')
+                    (tup_2 (indpred_decomp (a_convert_all_f constr vs))) Halltup2))
               (ltac:(intros; apply term_rep_irrel))
               (proj1' (pred_val_inv Hty4))
               (proj1' (proj2' (pred_val_inv Hty4)))
-              (proj2' (proj2' (pred_val_inv Hty4)))); auto.
-            Unshelve. all: auto.
+              (proj2' (proj2' (pred_val_inv Hty4)))).
+            (*Giving Hj' explicitly fails for some reason*)
+            Unshelve. 2: exact Hj'.
+            (*Simplify the casts*)
             rewrite rewrite_dom_cast.
             rewrite !dom_cast_compose.
-            (*We know that nothing in ps can appear, so we can switch interp*)
-            erewrite tm_change_pf with(p2:=pf); auto.
-            2: {
-              intros. simpl. rewrite find_apply_pred_notin; auto.
-              intro C. revert H0.
-              apply (get_indprop_args_pos _ _ Hposa Hinda); auto.
-              apply nth_In; auto.
-              inversion Hty4; subst; lia.
-            }
-            (*Now simplify RHS*)
+            (*Now, we must show that the term_reps are equal
+              under these valuations. This will take several steps.
+              First, assert the claim and simplify the casts*)
             symmetry.
-            
-            
-            rewrite tm_change_vv with(v2:=(substi_multi_let gamma_valid pd
-            (interp_with_Ps gamma_valid pd pf (map fst (get_indpred l)) Ps) vt
-            (substi_mult' vt vv (tup_1 (indpred_decomp (a_convert_all_f constr vs))) h')
-            (tup_2 (indpred_decomp (a_convert_all_f constr vs))) Halltup2)).
-            (*Casting is annoying*)
-            + assert (Htyeq: (snd (nth j vs vs_d)) = 
+            rewrite (tm_change_vv) with(v2:=
+              (substi_multi_let gamma_valid pd pf vt
+              (substi_mult' vt vv (tup_1 (indpred_decomp (a_convert_all_f constr vs))) h')
+              (tup_2 (indpred_decomp (a_convert_all_f constr vs))) Halltup2)).
+            {
+              (*Handle casting here*)
+              assert (Htyeq: (snd (nth j vs vs_d)) = 
               (ty_subst (s_params p') (map vty_var (s_params p')) (nth j (s_args p') vty_int))).
               {
                 eapply Typechecker.term_has_type_unique.
                 apply (proj2' (typed_eq_inv Hvalfeq)).
-                apply Hty2.
+                apply  (arg_list_hnth_ty (proj1' (pred_val_inv Hty4))
+                (proj2' (proj2' (pred_val_inv Hty4))) Hj').
               }
               match goal with | |- context [dom_cast ?pd ?Heq ?d] =>
                 generalize dependent Heq end.
@@ -2841,334 +3138,70 @@ Proof.
               assert (Heqr = eq_refl) by (apply UIP_dec; apply sort_eq_dec).
               subst. unfold dom_cast; simpl.
               apply term_rep_irrel.
-            + (*And now we prove these valuations are the same*)
-              (*TODO: START*)
-              intros x Hinfv.
-              rewrite substi_multi_let_change_pf with(pf1:=
-              (interp_with_Ps gamma_valid pd pf (map fst (get_indpred l)) Ps))
-              (pf2:=pf); simpl; auto.
-              * assert (Halltup2 = Hallval2) by (apply proof_irrel).
-                rewrite H0. f_equal.
-                f_equal.
-                (*TODO: better*)
-                apply functional_extensionality_dep; intros x'.
-                rewrite substi_multi_let_change_pf with(pf1:=
-              (interp_with_Ps gamma_valid pd pf (map fst (get_indpred l)) Ps))
-              (pf2:=pf); simpl; auto.
-              
-              proof_irrel.
-
-              Check Hallval2.
-              Check Halltup2.
-              f_equal. 
-              assert (Hnotinx1: ~ In x (map fst (tup_2 (indpred_decomp (a_convert_all_f constr vs))))).
-              {
-                intros Hinx.
-                Search 
-              }
-              (*This is because we used all new variables*)
-              rewrite !substi_multi_let_notin.
-
-              
-              
-            
-            generalize dependent (eq_trans Heq
-            (eq_trans
-               (cast_nth_eq (Hacast p' fs' (map (v_subst vt) (map vty_var (s_params p'))) e) j
-                  s_int) (substi_mult_nth_lemma (v_subst vt) snd vs j Hj s_int vs_d))).
-            generalize dependent (v_subst vt (snd (nth j vs vs_d))).
-            )
-            (*Now we can prove this*)
-            Check (eq_trans Heq
-            (eq_trans
-               (cast_nth_eq (Hacast p' fs' (map (v_subst vt) (map vty_var (s_params p'))) e) j
-                  s_int) (substi_mult_nth_lemma (v_subst vt) snd vs j Hj s_int vs_d))).
-            apply dom_cast_eq.
-              rewrite (get_indprop_args_length Hinda).
-              Search get_indprop_args.
-              eapply get_indprop_args_pos. apply H
-              intro C.
-              apply (get_indprop_args_pos .
-              (*TODO: before*)
-              assert (Hposf: ind_positive (map fst (get_indpred l)) constr). {
-                Search ind_positive.
-                rewrite Forall_forall in Hpos.
-                specialize (Hpos fs Hinfs').
-                rewrite Forall_forall in Hpos.
-                apply Hpos; auto.
-              } 
-              assert (Hvalinda:=(a_convert_all_f_valid_ind_form p f nil Hvalindf)).
-              assert (Hwfa:=(a_convert_all_f_wf f nil)).
-              assert (Hposa:=(a_convert_all_f_pos (map fst indpred) f nil Hposf)).
-              Search ind_strictly_positive.
-              
-              rewrite  unfold interp_with_Ps.
             }
-            (*Now we simplify the RHS*)
-
-            Check (eq_trans Heq
-            (eq_trans
-               (cast_nth_eq (Hacast p' fs' (map (v_subst vt) (map vty_var (s_params p'))) e) j
-                  s_int) (substi_mult_nth_lemma (v_subst vt) snd vs j Hj s_int vs_d))).
-
-            Search dom_cast scast.
-            rewrite fold_dom_cast.
-            with(Heq:=Heq)(Hty:=Hty2); auto.
-            erewrite get_arg_list_hnth.
-            Search hnth get_arg_list.
-            Search hnth cast_arg_list.
-
-
-            Unshelve.
-            Search substi_mult'.
-            Search tup_2.
-
-            Search substi_multi_let.
-            rewrite substi_multi_let_notin.
-
-
-
-
-            Check (ty_var_inv (proj1' (typed_eq_inv Hvalfeq))).
-          Unshelve.
-          2: {
-            inversion Handty; subst.
-            apply iter_fand_inv in H4.
-            Search iter_fand formula_typed.
-            ind_form_decomp:
-  forall (p : predsym) (f : formula),
-  valid_ind_form p f ->
-  tup_4 (indpred_decomp f) =
-  Fpred p (map vty_var (s_params p)) (snd (get_indprop_args f))
-
-            Search get_indprop_args.
-          }
-          Search iter_fand.
+            assert (Hincfs: In constr fs). {
+              unfold fs. rewrite in_map_iff. exists (name, constr); auto.
+            }
+            (*Now we prove that these valuations agree on the free
+              variables of a_i.
+              The key ideas: no var in vs occur in the original formula*)
+            intros x Hinxai.
+            (*See whether x occurs in let-bound vars or not*)
+            destruct (in_dec vsymbol_eq_dec x 
+              (map fst (tup_2 (indpred_decomp (a_convert_all_f constr vs))))).
+            + (*Case 1: x is in the let-bound vars*)
+              apply substi_multi_let_ext; auto.
+              apply tup_2_NoDup; auto.
+              (*Now prove that, for any free var in a 
+                let-bound term from tup_2,
+                the valuations are the same*)
+              intros y t1 Hint1 Hiny.
+              (*Again, see if y is in quantified vars or not
+                (either way similar)*)
+              destruct (in_dec vsymbol_eq_dec y (tup_1 (indpred_decomp (a_convert_all_f constr vs)))).
+              * (*If y in quantified vars, easy (bceause h' used both times!)*)
+                destruct (In_nth _ _ vs_d i1) as [k [Hk Hy]]; subst.
+                rewrite !substi_mult_nth' with(Hi:=Hk); auto;
+                apply tup_1_NoDup; auto.
+              * (*If not, push through to next layer, use fact that
+                  y CANNOT be in vs because vs not in constr*)
+                rewrite !substi_mult_notin; auto.
+                (*TODO: prove that all free vars in decomp
+                  are bound or free in original*)
+                intros Hiny2.
+                assert (Hinybnd: In y (fmla_bnd (a_convert_all_f constr vs))).
+                {
+                  apply tup_2_fv_closed with(t:=t1); auto.
+                  rewrite <- (alpha_closed constr) by
+                    apply a_convert_all_f_equiv.
+                  apply (constr_closed gamma_valid l_in Hinfs Hincfs).
+                }
+                apply (Hnotinvs y); auto.
+            + (*If x not in the the let-bound vars, we ignore
+              this binding and got to the next one*)
+              rewrite !substi_multi_let_notin; auto.
+              (*This time, see if x is in the quantified vars*)
+              destruct (in_dec vsymbol_eq_dec x (tup_1 (indpred_decomp (a_convert_all_f constr vs)))).
+              * (*If it is, we simplify and it is easy*)
+                destruct (In_nth _ _ vs_d i0) as [k [Hk Hy]]; subst.
+                rewrite !substi_mult_nth' with(Hi:=Hk); auto;
+                apply tup_1_NoDup; auto.
+              * (*Otherwise, we just need to show that x not in vs*)
+                rewrite !substi_mult_notin; auto.
+                intros Hinx2.
+                assert (Hinxbnd: In x (fmla_bnd (a_convert_all_f constr vs))).
+                {
+                  apply tup_4_fv_closed.
+                  -  rewrite <- (alpha_closed constr) by
+                    apply a_convert_all_f_equiv.
+                    apply (constr_closed gamma_valid l_in Hinfs Hincfs).
+                  - rewrite (ind_form_decomp p' _ Hinda). simpl.
+                    simpl_set. exists ((nth j (snd (get_indprop_args (a_convert_all_f constr vs))) tm_d)).
+                    split; auto. apply nth_In; auto.
+                    inversion Hty4; subst.
+                    rewrite H5; auto.
+                }
+                apply (Hnotinvs x); auto.
         }
-        Search 
-        Print substi_mult'.
-        Print substi_multi_let.
-        Search h'.
-
-
-
-          Search alpha_f_aux.
-          Search a_convert_all_f.
-        }
-          revert Hin. apply (gen_strs_notin.
-
-            Search sublist concat.
-          }
-
-          unfold vsymbol in *.
-          set (v1 := nth j (gen_strs (Datatypes.length (s_args p')) (concat (map fmla_bnd fs)))
-          ""%string) in *.
-          set (v:= (nth j (gen_strs (Datatypes.length (s_args p')) (concat (map fmla_bnd fs)))
-          ""%string, nth j (s_args p') vty_int) : vsymbol) in *.
-
-          assert 
-          apply gen_strs_notin with (n:=()).
-          intros Hin.
-          apply (gen_strs_notin )
-          [| rewrite gen_strs_length; auto].
-          Search gen_strs.
-        }
-        
-        Unshelve.
-        Search descend a_equiv_f.
-
-
-
-Search indpred_decomp.
-
-      
-      
-      
-      
-      (indpred_decomp f)))).
-
-
-
-      t_and_simp acc (Feq (snd v) (Tvar v) t) in
-    fold_left2 marry Ftrue vs tms
-
-        (*TODO: now we need to prove a decomposition theorem
-          for [descend vs f] and prove that we can translate
-          between them (use same decomp except for part 4,
-          prove equivalent),
-          so define descend_decomp =
-          fexists (tup_1 (indpred_decomp f))
-            (iter_flet (tup_2)...
-            then define new one for last,
-            or can define with (tup_4) and a translation to
-            a bunch of equalities)
-          think we will need to know that no vsymbol appears
-          from the list (myeb not - substi_mult
-          overwrite it - prove twice has no effect)*)
-
-
-
-        Unshelve.
-        apply add_axioms_sound.
-        
-        
-        
-        with(f:=).
-
-
-
-        Search get_hlist_elt.
-        subst Ps. simpl.
-
-
-
-        Lemma indpred_decomp_equiv (pf: pi_funpred gamma_valid pd) 
-  (vt: val_typevar) (vv: val_vars pd vt)  
-  (f: formula) (Hval: formula_typed gamma f)
-  (Hwf: fmla_wf f) :
-  formula_rep gamma_valid pd vt pf vv f Hval =
-  formula_rep gamma_valid pd vt pf vv 
-    (indpred_transform f) (indpred_transform_valid f Hval).
-
-
-        Print indpred_decomp.
-
-        Search In dep_map.
-        Search iter_and.
-
-
-
-        replace (cast_arg_list
-        (eq_trans (eq_trans (f_equal (map (v_subst vt)) Hmapsnd) (eq_sym Hsigma))
-           (Hacast p l0 (map (v_subst vt) (map vty_var (s_params p))) e)) h)
-        with h.
-        2: {
-
-        }
-        Search cast_arg_list.
-
-        case_in.
-
-
-        Search get_assoc_list.
-        simpl.
-      
-      Search get_hlist_elt.
-
-
-      cut Hleast.
-
-
-      prove_hyp Hleast.
-
-
-
-
-      Fixpoint gen_hlist {A: Type} (f: A -> Type) (g: forall (a: A), f a)
-  (l: list A) :
-  hlist f l :=
-  match l as l' return hlist f l' with
-  | nil => HL_nil _
-  | x :: xs => HL_cons _ x xs (g x) (gen_hlist f g xs)
-  end.
-
-Lemma gen_hlist_get_elt {A: Type}
-  (eq_dec: forall x y, {x = y} + {x <> y}) 
-  {f: A -> Type} {g: forall (a: A), f a} {l: list A} (x: A)
-  (Hinx: in_bool eq_dec x l):
-  get_hlist_elt eq_dec (gen_hlist f g l) x Hinx = g x.
-Proof.
-  induction l; simpl. inversion Hinx.
-  simpl in Hinx.
-  destruct (eq_dec x a); subst; auto.
-Qed.
-      (*function:
-        fun p srts a ->
-        formula_rep gamma_valid pd vt pf
-          (substi_mult' vt vv (create_vsymbols ...) (s_args p) a)
-        (map join_left Ftrue (exi (create_vsymbols ...)) (s_args p) t_or 
-          (ugh, need to get l0 - can but annoying - get_indconstrs p)
-        (ty_lemma)*)
-
-
-
-        Check (substi_mult' vt vv
-        (create_vsymbols (concat (map fmla_bnd (map snd l0))) (s_args p)) h
-        (nth i (create_vsymbols (concat (map fmla_bnd (map snd l0))) (s_args p)) vs_d)).
-
-        assert 
-
-
-        [|]
-        Unshelve.
-        Search hnth get_arg_list.
-        Search hnth cast_arg_list.
-
-
-        Unshelve.
-      }
-
-
-
-          map (v_subst vt)
-   (map snd (create_vsymbols (concat (map fmla_bnd (map snd l0))) (s_args p))) =
- sym_sigma_args p (map (v_subst vt) (map vty_var (s_params p)))"
-         )
-      Check constr_rep.
-      (*So the plan
-        1. prove that we can cast h (or redefine/reprove for now
-          fforalls_rep) to something of type
-          arg_list (dom_aux pd) (map (v_subst vt) (s_args p))
-        2. Prove that when we cast h' under Hsigma, we get 
-          [pred_arg_list...], can rewrite in Hp
-        3. Specialize Hleast with this casted h/h'/h''
-        4. Again, prove vt_with_args the same and rewrite (hope it works)
-        5. Define Ps - I believe we should have it so
-          that the ith element is fun a => 
-            formula_rep of (join exi ... )
-            under valuation where vs are sent to a (substi_mult, as above)
-            so exactly as given here just generalized
-        6. Easy to show then that this is [get_hlist_elt]
-        7. Remaining, show constructors are satisfied
-          *)
-      rewrite Hsigma in Hleast.
-        
-        rewrite !map_length; auto.
-
-        2: {}
-        2: { rewrite ty_subst_fun_notin; auto. }
-
-        rewrite ty_subst_fun_params_id.
-        rewrite ty_subst_s_nth.
-        Search map vty_var.
-
-      }
-      Check cast_arg_list.
-      assert (Hheq: )
-
-      generalize dependent h.
-      unfold create_vsymbols. rewrite map_snd_combine.
-      unfold create_vsymbols in h.
-      rewrite map_snd_combine in h.
-      assert (Hargseq: forall Heq, (pred_arg_list pd vt p (map vty_var (s_params p))
-      (map Tvar (create_vsymbols (concat (map fmla_bnd (map snd l0))) (s_args p)))
-      (term_rep gamma_valid pd vt pf
-         (substi_mult pd vt vv
-            (create_vsymbols (concat (map fmla_bnd (map snd l0))) (s_args p)) h))
-      (proj1' (typed_binop_inv Hty1))) = scast Heq h).
-
-      (*We already know the arg list a*)
-      
-      (*TODO: remove fs from this*)
-      (map snd l0)).
-      
-      apply fforalls_typed_inv in Hty.
-        apply Hty. }
-      simpl. Search fforalls formula_typed. }
-      Unshelve.
-      2: {
-        apply gen_axioms_typed. auto.
-
-      }
-      rewrite fforalls_rep.
-      Unshelve.
+        (*Now we are just left with proving all of the
+          antecedents, for which we need a separate lemma*)
